Further constructive approach definitions - Requires rewrites of FOL part to stick closer to ModelTheory and get rid of RTR system, by using term equality, ordering, projection as restriction? and renaming as relabeling?

RelationalAlgebra/Equivalence.lean
@@ -2,6 +2,51 @@ import RelationalAlgebra.RA.Query
 import RelationalAlgebra.FOL.Evaluate
 
 open RM
+def att_to_var : Attribute → FOL.Variable :=
+  Nat.repr
+
+def var_to_att : FOL.Variable → Attribute :=
+  String.toNat!
+
+theorem var_to_att_to_var_eq_id : var_to_att ∘ att_to_var = id := by
+  sorry
+
+def schema_to_inFn {n} (dbs : DatabaseSchema) (rn : RelationName) : Attribute →. FOL.Language.fol.Term (FOL.Variable ⊕ Fin n) :=
+  PFun.res (FOL.outVar ∘ att_to_var) (dbs rn)
+
+def ra_to_fol_R {dbi} (rn : RelationName) : FOL.EvaluableQuery dbi := ⟨
+  .R ⟨⟨schema_to_inFn dbi.schema rn, rn, by apply Fintype.ofFinset (dbi.schema rn); simp_all [PFun.res, schema_to_inFn]⟩, dbi, by simp_all [schema_to_inFn, PFun.res]; aesop⟩,
+  PFun.res att_to_var (dbi.schema rn),
+  by
+    apply Fintype.ofFinset (dbi.schema rn);
+    simp_all [PFun.res]
+  ,
+  by
+    simp_all [PFun.ran, FOL.BoundedQuery.variablesInQuery, FOL.RelationTermRestriction.outVars, FOL.RelationTermRestriction.vars, FOL.outVar?, att_to_var, schema_to_inFn, FOL.outVar, Finset.filterMap, PFun.res, PFun.restrict, Part.restrict]
+    ext v
+    simp_all only [Set.mem_toFinset, Set.mem_setOf_eq, Part.mem_mk_iff, Finset.mem_coe, exists_prop, Finset.mem_mk,
+      Multiset.mem_filterMap, Finset.mem_val, exists_exists_and_eq_and]
+    apply Iff.intro
+    · intro a
+      obtain ⟨w, h⟩ := a
+      obtain ⟨left, right⟩ := h
+      subst right
+      apply Exists.intro
+      · apply And.intro
+        on_goal 2 => {rfl
+        }
+        · simp_all only
+    · intro a
+      obtain ⟨w, h⟩ := a
+      obtain ⟨left, right⟩ := h
+      simp_all only [FOL.outVar?, Sum.getLeft?_inl, Option.some.injEq]
+      subst right
+      apply Exists.intro
+      · apply And.intro
+        on_goal 2 => {rfl
+        }
+        · simp_all only
+⟩
 
 def ra_to_fol_s {dbi} (w : FOL.EvaluableQuery dbi) (a : Attribute) (b : Attribute ⊕ Value) (posEq : Bool) : FOL.EvaluableQuery dbi := ⟨
   w.query,
@@ -10,16 +55,115 @@ def ra_to_fol_s {dbi} (w : FOL.EvaluableQuery dbi) (a : Attribute) (b : Attribut
   by sorry
 ⟩
 
+theorem p_sub_query_proof {rs dbi} {w : FOL.EvaluableQuery dbi} (h : ↑rs ⊆ w.schema) : ↑rs ⊆ w.outFn.Dom := by simp_all [FOL.EvaluableQuery.schema]
+
+def emptyRTR {n} (name : RelationName): FOL.RelationTermRestriction n := ⟨(λ _ => .none), name, (by apply Fintype.ofFinset ∅; simp_all)⟩
+
+def freeVarRTR (name : RelationName) (rs : RelationSchema) (att : Attribute) (h : att ∈ rs.ordering) : FOL.RelationTermRestriction rs.card := ⟨
+    (λ a => ite (a = att) ((rs.index? att).map FOL.inVar) (.none)),
+    name,
+    by
+      apply Fintype.ofFinset {att}
+      intro x
+      simp_all only [Finset.mem_singleton, PFun.dom_mk, Set.mem_setOf_eq]
+      apply Iff.intro
+      · intro a
+        subst a
+        simp_all only [RelationSchema.ordering_mem, ↓reduceIte, Part.ofOption_dom, Option.isSome_map',
+          RelationSchema.index?_isSome]
+      · intro a
+        split at a
+        next h =>
+          subst h
+          simp_all only [Part.ofOption_dom, Option.isSome_map', RelationSchema.index?_isSome_eq_iff]
+        next h => simp_all only [Part.not_none_dom]
+⟩
+
+def FOL.RelationTermRestriction.merge {n} (prev added : FOL.RelationTermRestriction n) : FOL.RelationTermRestriction n := ⟨
+  λ a => ite (prev.inFn a).Dom (prev.inFn a) (added.inFn a),
+  prev.name,
+  by
+    apply Fintype.ofFinset (prev.inFn.Dom.toFinset ∪ added.inFn.Dom.toFinset)
+    intro x
+    simp_all only [Finset.mem_union, Set.mem_toFinset, PFun.mem_dom, PFun.dom_mk, Set.mem_setOf_eq]
+    apply Iff.intro
+    · intro a
+      cases a with
+      | inl h =>
+        obtain ⟨w, h⟩ := h
+        split
+        next h_1 => simp_all only
+        next h_1 => rw [Part.dom_iff_mem] at h_1; simp_all
+      | inr h_1 =>
+        obtain ⟨w, h⟩ := h_1
+        split
+        next h_1 => simp_all only
+        next h_1 => rw [Part.dom_iff_mem]; use w
+    · intro a
+      split at a
+      next h =>
+        simp_all only
+        rw [Part.dom_iff_mem] at a; simp_all
+      next h => rw [Part.dom_iff_mem] at a; simp_all
+⟩
+
+-- Use ordering, otherwise we require comm and assoc for merge :(
+def FOL.RelationTermRestriction.project {n} (rtr : FOL.RelationTermRestriction n) (rs : RelationSchema) : FOL.RelationTermRestriction rs.card :=
+  rs.ordering.foldl (λ prev (a : Attribute) => dite (a ∈ rs.ordering) (λ h => FOL.RelationTermRestriction.merge (freeVarRTR rtr.name rs a h) prev) (λ _ => prev)) (emptyRTR rtr.name)
+
+theorem FOL.RelationTermRestriction.merge_name {n} (prev added : FOL.RelationTermRestriction n) (h : prev.name = added.name)
+  : (FOL.RelationTermRestriction.merge prev added).name = prev.name := by
+    simp_all only
+    exact h
+
+theorem FOL.RelationTermRestriction.project_name {n} (rtr : FOL.RelationTermRestriction n) (rs : RelationSchema)
+  : (FOL.RelationTermRestriction.project rtr rs).name = rtr.name := by
+    simp_all [project]
+    induction rs using Finset.induction with
+    | empty => simp_all only [Finset.card_empty, Finset.not_mem_empty, ↓reduceDIte, List.foldl_fixed, emptyRTR]
+    | insert h_new ih =>
+      simp_all
+      rename_i a s
+      by_cases h : a ∈ s
+      . sorry
+      . sorry
+
+def FOL.BoundedQuery.wrapEx {n} (sq : FOL.BoundedQuery m) (m : ℕ) (h : n ≤ m) : FOL.BoundedQuery n :=
+  dite (m = n) (λ _ => sq.cast n) (λ h2 => .ex (sq.wrapEx (m) (by apply Nat.succ_le_of_lt; exact Nat.lt_of_le_of_ne h fun a ↦ h2 (id (Eq.symm a)))))
+
+def FOL.BoundedRelationTermRestriction.projectBRTR {n} (brtr : FOL.BoundedRelationTermRestriction n) (rs : RelationSchema) (h : n ≤ rs.card) : FOL.BoundedQuery n :=
+  (FOL.BoundedQuery.R ⟨(⟨brtr.inFn, brtr.name, brtr.fintypeDom⟩ : RelationTermRestriction n).project rs, brtr.dbi, by simp_all [FOL.RelationTermRestriction.project]⟩).wrapEx rs.card h
+
+
+def FOL.BoundedQuery.project {n} : FOL.BoundedQuery n → RelationSchema → FOL.BoundedQuery n
+  | .R brtr, rs => brtr.projectBRTR rs (by sorry)
+  | q, _ => q
+
+def ra_to_fol_p {dbi} (w : FOL.EvaluableQuery dbi) (rs : RelationSchema) (h : ↑rs ⊆ w.schema) : FOL.EvaluableQuery dbi := ⟨
+  w.query.project rs,
+  w.outFn.restrict (p_sub_query_proof h),
+  by
+    apply Fintype.ofFinset rs
+    intro x
+    simp [FOL.EvaluableQuery.schema] at h
+    simp_all only [PFun.mem_dom, PFun.mem_restrict, Finset.mem_coe, exists_and_left, iff_self_and]
+    intro a
+    have z : x ∈ w.outFn.Dom := by apply Set.mem_of_subset_of_mem h a
+    simp_all only [PFun.mem_dom]
+  ,
+  by
+    simp_all [PFun.ran, FOL.BoundedQuery.project]
+    ext v
+    sorry
+⟩
+
 noncomputable def ra_to_fol_r {dbi} (w : FOL.EvaluableQuery dbi) (f : Attribute → Attribute) (h : f.Bijective) : FOL.EvaluableQuery dbi := ⟨
   w.query,
   w.outFn ∘ f.invFun,
   by
-    have z : w.outFn.Dom.Finite := Set.toFinite w.outFn.Dom
-    apply Set.Finite.fintype
-    simp_all [PFun.Dom, Part.dom_iff_mem]
-    apply Set.Finite.ofFinset (z.image f).toFinset
+    apply Fintype.ofFinset (w.outFn.Dom.toFinset.image f);
     intro x
-    simp_all only [Set.Finite.mem_toFinset, Set.mem_image, Set.mem_setOf_eq]
+    simp_all only [Finset.mem_image, Set.mem_toFinset, PFun.mem_dom, Function.comp_apply]
     apply Iff.intro
     · intro a
       obtain ⟨w_1, h_1⟩ := a
@@ -50,21 +194,127 @@ noncomputable def ra_to_fol_r {dbi} (w : FOL.EvaluableQuery dbi) (f : Attribute 
 
 noncomputable def ra_to_fol_def [FOL.folStruc] {dbi} (raQ : RA.Query) (h : raQ.isWellTyped dbi.schema) : FOL.EvaluableQuery dbi :=
   match raQ with
+  | .R rn => ra_to_fol_R rn
+  | .s a b pos sq => ra_to_fol_s (ra_to_fol_def sq (by simp_all [RA.Query.isWellTyped])) a b pos
+  | .p rs sq => ra_to_fol_p (ra_to_fol_def sq (by simp_all [RA.Query.isWellTyped])) rs (by simp [RA.Query.isWellTyped] at h; aesop?)
+  -- | .j sq1 sq2 => ra_to_fol_j (ra_to_fol_def sq1 (by simp_all [RA.Query.isWellTyped])) (ra_to_fol_def sq2 (by simp_all [RA.Query.isWellTyped])) sq1 sq2
   | .r f sq => ra_to_fol_r (ra_to_fol_def sq (by simp_all [RA.Query.isWellTyped])) f (by simp_all [RA.Query.isWellTyped])
   | _ => sorry
 
 theorem ra_to_fol_eval [FOL.folStruc] {dbi} (raQ : RA.Query) (h : raQ.isWellTyped dbi.schema) :
   raQ.evaluate dbi h = (ra_to_fol_def raQ h).evaluate := by
     simp [FOL.EvaluableQuery.evaluate, RA.Query.evaluate, FOL.EvaluableQuery.schema]
-    induction raQ with
-    | r f sq ih =>
+    induction raQ
+    all_goals (
       simp only [RA.Query.isWellTyped] at h
+      simp_all only [FOL.EvaluableQuery.evaluateT, forall_true_left, RA.Query.schema, ra_to_fol_def, RA.Query.evaluateT]
+    )
+    case R rn =>
       apply And.intro
-      . simp_all only [RA.Query.schema, renameSchema]
-        simp_all only [ra_to_fol_def, ra_to_fol_r]
+      . simp_all [ra_to_fol_R, PFun.res, PFun.restrict, PFun.Dom, Part.restrict]
+      . simp_all [ra_to_fol_R]
+        ext t
+        simp_all only [Set.mem_setOf_eq]
+        apply Iff.intro
+        · intro ht
+          use λ v => t (var_to_att v)
+          apply And.intro
+          · simp_all [FOL.Query.Realize]
+            apply And.intro
+            · sorry
+            · apply And.intro
+              · sorry
+              · simp [PFun.ran]
+          · unfold FOL.VariableAssignmentToTuple
+            simp_all [PFun.res, PFun.restrict, Part.restrict, Part.bind]
+            simp [← Function.comp_apply, var_to_att_to_var_eq_id]
+            simp_all only [Function.comp_apply]
+            ext a v
+            simp_all only [Part.mem_assert_iff, Finset.mem_coe, exists_prop, iff_and_self]
+            intro a_1
+            rw [DatabaseInstance.validSchema]
+            have hz : a ∈ t.Dom → a ∈ (dbi.relations rn).schema := by simp [(dbi.relations rn).validSchema t ht]
+            apply hz
+            apply (PFun.mem_dom t a).mpr
+            use v
+        · intro a
+          obtain ⟨w, h⟩ := a
+          obtain ⟨left, right⟩ := h
+          subst right
+          sorry
+    case s a b posEq sq ih =>
+      apply And.intro
+      . simp_all only [ra_to_fol_s, Set.toFinset_inj]
+      . simp_all [ra_to_fol_s, selectionT]
+        ext t
+        simp_all only [Set.mem_setOf_eq]
+        apply Iff.intro
+        . intro a_1
+          obtain ⟨left_3, right_2⟩ := a_1
+          obtain ⟨w, h⟩ := left_3
+          use w
+          simp_all only [true_and]
+          rfl
+        . unfold FOL.VariableAssignmentToTuple at *
+
+          intro a_1
+          simp_all only [true_and]
+          obtain ⟨left, right⟩ := h
+          obtain ⟨left_1, right⟩ := right
+          obtain ⟨left_2, right_1⟩ := ih
+          obtain ⟨w, h⟩ := a_1
+          obtain ⟨left_3, right_2⟩ := h
+          subst right_2
+          simp_all only
+          cases b with
+          | inl val =>
+            simp_all only [selectionT.def_att]
+            split
+            next h =>
+              subst h
+              ext v
+              simp_all only [Part.mem_bind_iff]
+              apply Iff.intro
+              · intro a_1
+                obtain ⟨w_1, h⟩ := a_1
+                obtain ⟨left_4, right_2⟩ := h
+                sorry
+              · intro a_1
+                obtain ⟨w_1, h⟩ := a_1
+                obtain ⟨left_4, right_2⟩ := h
+                sorry
+            next h =>
+              simp_all only [Bool.not_eq_true]
+              subst h
+              apply Aesop.BuiltinRules.not_intro
+              intro a_1
+              sorry
+          | inr val_1 =>
+            simp_all only [selectionT.def_val]
+            split
+            next h =>
+              subst h
+              ext v
+              simp_all only [Part.mem_bind_iff, Part.mem_some_iff]
+              apply Iff.intro
+              · intro a_1
+                obtain ⟨w_1, h⟩ := a_1
+                obtain ⟨left_4, right_2⟩ := h
+                sorry
+              · intro a_1
+                subst a_1
+                sorry
+            next h =>
+              simp_all only [Bool.not_eq_true]
+              subst h
+              apply Aesop.BuiltinRules.not_intro
+              intro a_1
+              sorry
+    case r f sq ih =>
+      apply And.intro
+      . simp_all only [renameSchema, ra_to_fol_r]
         aesop
-      . simp_all [RA.Query.evaluateT, renameT]
-        simp_all [ra_to_fol_def, ra_to_fol_r, FOL.EvaluableQuery.evaluateT, FOL.VariableAssignmentToTuple]
+      . simp_all only [renameT, Set.mem_setOf_eq, exists_eq_right', ra_to_fol_r]
         ext t
         simp_all only [forall_true_left, Set.mem_setOf_eq]
         obtain ⟨left, right⟩ := h
@@ -75,10 +325,9 @@ theorem ra_to_fol_eval [FOL.folStruc] {dbi} (raQ : RA.Query) (h : raQ.isWellType
           obtain ⟨left_2, right_2⟩ := h
           use w
           simp_all only [true_and]
-          unfold FOL.VariableAssignmentToTuple at ⊢ right_2 right_1
-          simp_all only [Function.comp_apply]
           ext a v
-          simp_all only [Part.mem_bind_iff]
+          unfold FOL.VariableAssignmentToTuple at *
+          simp_all only [Function.comp_apply, Part.mem_bind_iff]
           apply Iff.intro
           · intro a_1
             sorry
@@ -96,7 +345,7 @@ theorem ra_to_fol_eval [FOL.folStruc] {dbi} (raQ : RA.Query) (h : raQ.isWellType
             · exact left_2
             · ext a b : 1
               simp_all only [Function.comp_apply, inv_f_id_apply, Part.mem_bind_iff]
-    | _ => sorry
+    all_goals sorry
 
 
 theorem ra_to_fol [FOL.folStruc] {dbi} (raQ : RA.Query) (h : raQ.isWellTyped dbi.schema) :
